\mysection{Differentialregning}
Den afledede af $f$ skrives som $f'=\frac{d}{dx}f=\frac{df}{dx}$.
\textcolor{white}{hemmelig tekst}

\mysubsection{Regneregler}
Der gælder at
\begin{center}
		\begin{tabular}{@{}l l@{}}
		$f(x)$      & $f'(x)$  				\\ \toprule
		$c$			& $0$ 					\\ \midrule
		$x$			& $1$					\\ \midrule
		$x^n$  		& $nx^{n-1}$			\\ \midrule
		$e^x$  		& $e^x$					\\ \midrule
		$e^{cx}$  	& $ce^{cx}$				\\ \midrule
		$a^x$  		& $a^x\ln a $			\\ \midrule
		$\ln x$ 	& $\frac{1}{x}$			\\ \midrule
		$\cos x$  	& $-\sin x$				\\ \midrule
		$\sin x$  	& $\cos x$				\\ \midrule
		$\tan x$ 	& $1+\tan^2(x)$		\\ \bottomrule  
	\end{tabular}
\end{center}
\mysubsection{Generelle regneregler}
Der gælder at
\begin{align*}
&(cf)'(x)=cf'(x)\\
&(f\pm g)'(x)=f'(x)\pm g'(x)\\
&(fg)'(x)=f'(x)g(x)+f(x)g'(x)\\
&\Big(\frac{f}{g}\Big)'(x)=\frac{f'(x)g(x)-f(x)g'(x)}{g^2(x)}\\
&\frac{d}{dx}f(g(x))=f'(g(x))g'(x).
\end{align*}
Den sidste regneregel kaldes \emph{kædereglen}.