\newpage
\section{Math101 answers}
\begin{enumerate}

	\item The answers are:
	\begin{align*}
	f_1'(x)=\frac{x}{\sqrt{x^2+1}},&& f_2'(x)=\frac{1}{(2x+1)^2},&& f_3'(x)=\sin(x)+x\cos(x).
	\end{align*}

	\item The answers are:
	\begin{align*}
	f_1'(x)=(x+1)e^x,&& f_2'(x)=4x\cos(x)-2x^2\sin(x),\\ f_3'(x)=(\frac{1}{x}+\ln(x))e^x,&& f_4'(x)=\cos^2(x)-\sin^2(x).
	\end{align*}

	\item The answers are:
	\begin{align*}
	f_1'(x)=\frac{-1}{(x-1)^2},&&f_2'(x)=\frac{3x^2+4x-5}{(3x+2)^2},&&f_3'(x)=\frac{-1}{(x-2)^2}.
	\end{align*}
	
	\item The answers are:
	\begin{align*}
	f_1'(x)=4(3x-1)^\frac{1}{3},&& f_2'(x)=\frac{2x+3}{x^2+3x},&& f_3'(x)=-e^{2-x},&&f_4'(x)=3x^2\cos(x^3).
	\end{align*}
	
	\item \label{it:diff24} The answer is $f'(x)=xe^x$.
	
	
	\item \label{it:diff23} The answer is $f'(x)=\ln(x)$.
	
	\item The answers are:
	\begin{align*}
	f_1'(x)=3x^2e^{x^3},&&f_2'(x)=-2\cos(x)\sin(x),\\f_3'(x)=3\sin^2(x)\cos(x)&&f_4'(x)=4x(1+\tan^2(x^2)).
	\end{align*}
		
	\item\label{it:diff21} We have that 
	\begin{align*}
	\frac{d}{dx} \frac{\sin(x)}{\cos(x)}=\frac{\cos^2(x)+\sin^2(x)}{\cos^2(x)}=1+\tan^2(x).
	\end{align*}

	\item The answer is $f'(x)=\frac{(x+1)e^x\cos(x)-xe^x\sin(x)}{\cos^2(x)}$.
		
	\item The answers are:
	\begin{align*}
	f'(x)=-2\cos(\sqrt{x^2+1})\sin(\sqrt{x^2+1})\frac{x}{\sqrt{x^2+1}}.
	\end{align*}
		
	\item The answers are:
	\begin{align*}
	f_1'(x)=\frac{2\cos(x)\sin^2(x)-\cos^3(x)}{\sin^2(x)},&&f_2'(x)=\frac{(2x^2-1)e^{x^2}}{x^2},\\f_3'(x)= \frac{(1-x)\cos(x)-x\sin(x)}{e^{x}}
	\end{align*}
	
	
	
	\item The answers are:
	\begin{align*}
	f(x)&=\frac{(-(x+1)\ln(x)+1)e^x}{\ln^2(x)},\\ g(x)&=e^x((1+x)\ln (x)+1),\\ h(x)&=xe^x((2+x)\sin(x)+x\cos(x)) )
	\end{align*}
	
	
\end{enumerate}